\section{}
Using index notation, prove the following expression is true:
\begin{equation*}
    (\vec{a} \times \vec{b}) \times (\vec{c} \times \vec{d}) = \vec{c}[ \vec{d} \cdot (\vec{a} \times \vec{b})] - \vec{d}[ \vec{c} \cdot (\vec{a} \times \vec{b})]
\end{equation*}
Use index notation and replace the indices only at the end.

\subsection*{Solution}
Similar to Question 1, expand LHS,
\begin{align*}
    %(\vec{a} \times \vec{b}) \times (\vec{c} \times \vec{d}) &= C_i \
    \underbrace{(\vec{a} \times \vec{b})}_{P_j} \times \underbrace{(\vec{c} \times \vec{d})}_{Q_k} &= \epsilon_{ijk} P_j Q_k \\
    &= \epsilon_{ijk} P_j (\epsilon_{klm} c_l d_m) \\
    &= \epsilon_{ijk} \epsilon_{klm} P_j c_l d_m \\
    &= (\delta_{il} \delta_{jm} - \delta_{im} \delta_{jl}) P_j c_l d_m \\
    &= (\delta_{il} \delta_{jm} P_j c_l d_m) - (\delta_{im} \delta_{jl} P_j c_l d_m) \\
    &= (P_j c_i d_j) - (P_j c_j d_i) \\
    &= c_i [d_j P_j] - d_i [c_j P_j] \\
    &= \vec{c} [ \vec{d} \cdot (\vec{a} \times \vec{b})] - \vec{d} [ \vec{c} \cdot (\vec{a} \times \vec{b})] \qed
\end{align*}    